proof progress on theorem 2

thm2_TEMP.thy
@@ -46,8 +46,32 @@ shows "(conf_sin \<epsilon> angleOutputE AnglePIDANN AnglePID_C)"
 definition spec_f :: "real \<Rightarrow> real \<Rightarrow> real" where
 "spec_f x_1 x_2 = (P * x_1) + (D * x_2)"
 
-definition spec_f_single :: "real \<Rightarrow> real" where
-"spec_f_single x_1 = (P * x_1)"
+
+definition norm_spec_f :: "real \<Rightarrow> real \<Rightarrow> real" where 
+"norm_spec_f x_1 x_2 = (denormI 1 (x_1 * P) + (denormI 2 (x_2 * D) ))"
+
+definition norm_spec_f_2 :: "real \<Rightarrow> real \<Rightarrow> real" where 
+"norm_spec_f_2 x_1 x_2 = 
+  (P * denormI 1 (x_1) + (D * denormI 2 (x_2)) )"
+
+lemma norm_spec_f_mono: 
+  fixes x_1 :: real and x_2 :: real and y_1 :: real and y_2 :: real
+  assumes "P > 0" and "D > 0" and 
+    "(snd(inRanges(1)) > fst(inRanges(1)) \<and> snd(inRanges(2)) > fst(inRanges(2)) \<and> snd(annRange) > fst(annRange))"
+  shows "x_1 \<le> y_1 \<and> x_2 \<le> y_2 \<longrightarrow> (norm_spec_f x_1 x_2) \<le> (norm_spec_f y_1 y_2)"
+  using assms apply (simp add: mono_denormI mono_norm norm_spec_f_def ordered_ab_semigroup_add_class.add_mono)
+  by (smt (verit, best) One_nat_def assms(3) mono_denormI mult.commute mult_left_mono)
+ 
+
+lemma norm_spec_f_2_mono: 
+  fixes x_1 :: real and x_2 :: real and y_1 :: real and y_2 :: real
+  assumes "P > 0" and "D > 0" and 
+    "(snd(inRanges(1)) > fst(inRanges(1)) \<and> snd(inRanges(2)) > fst(inRanges(2)) \<and> snd(annRange) > fst(annRange))"
+  shows "x_1 \<le> y_1 \<and> x_2 \<le> y_2 \<longrightarrow> (norm_spec_f_2 x_1 x_2) \<le> (norm_spec_f_2 y_1 y_2)"
+  using assms apply (simp add: mono_denormI mono_norm norm_spec_f_def mono_normI
+            ordered_ab_semigroup_add_class.add_mono)
+  by (smt (verit, best) assms(3) mono_denormI mono_normI mult.commute mult_le_cancel_left_pos norm_spec_f_2_def)
+  
 
 lemma spec_f_mono: 
   fixes x_1 :: real and x_2 :: real and y_1 :: real and y_2 :: real
@@ -62,6 +86,7 @@ term "[ ((normI 1 (inRanges(1).1)), ((normI 1 (inRanges(1).2)))),
 definition int :: "(real \<times> real) list" where
 "int = [ ((normI 1 (inRanges(1).1)), ((normI 1 (inRanges(1).2)))), 
          ((normI 2 (inRanges(2).1)), ((normI 2 (inRanges(2).2)))) ]"
+term "#int"
 
 (*Using FST for MIN and SND for MAX, when encoding the intervals. *)
 term "fst(int(1))"
@@ -92,7 +117,7 @@ lemma spec_mono_ann:
           "fst(int(1)) \<le> x_1 \<and> x_1 \<le> snd(int(1))" and 
           "fst(int(2)) \<le> x_2 \<and> x_2 \<le> snd(int(2))" and 
           "(snd(outRanges ! 0) > fst(outRanges ! 0) \<and> snd(annRange) > fst(annRange))" and
-          "\<epsilon> > 0" and 
+          "\<epsilon> \<ge> 0" and 
           "P > 0 \<and> D > 0" and
           "f_ann x_1 x_2 \<le> normO 1 (S (fst(int(1))) (fst(int(2))) + \<epsilon>)
                \<and> f_ann x_1 x_2 \<ge> normO 1 (S (snd(int(1))) (snd(int(2))) - \<epsilon>) 
@@ -119,7 +144,7 @@ proof (rule conjI)
         normO 1 ((S x_1 x_2) + \<epsilon>) \<ge> normO 1 ((S (fst(int(1))) (fst(int(2)))) + \<epsilon>)"
     using assms 
     apply (simp add: mono_normO)
-    by (smt (verit, ccfv_SIG) One_nat_def mono_normO)
+    by (smt (verit, ccfv_SIG) diff_Suc_1 mono_normO)
   from 1 c1 show "f_ann x_1 x_2 \<le> normO 1 ((S x_1 x_2) + \<epsilon>)"
     using \<open>fst (thm2_TEMP.int(1)\<^sub>s) \<le> x_1 \<and> fst (thm2_TEMP.int(2)\<^sub>s) \<le> x_2\<close> \<open>fst (thm2_TEMP.int(2)\<^sub>s) \<le> x_2 \<longrightarrow> S (fst (thm2_TEMP.int(1)\<^sub>s)) (fst (thm2_TEMP.int(2)\<^sub>s)) \<le> S x_1 x_2\<close> by argo
     
@@ -135,10 +160,20 @@ proof (rule conjI)
         normO 1 ((S x_1 x_2) - \<epsilon>) \<le> normO 1 ((S (snd(int(1))) (snd(int(2)))) - \<epsilon>)"
     using assms 
     apply (simp add: mono_normO)
-    by (smt (verit, best) One_nat_def mono_normO)
+    by (smt (verit, ccfv_SIG) diff_Suc_1 mono_normO)
   from 2 c2 show "f_ann x_1 x_2 \<ge> (normO 1 (S (x_1) (x_2) - \<epsilon>))"
     using \<open>x_1 \<le> snd (thm2_TEMP.int(1)\<^sub>s) \<and> x_2 \<le> snd (thm2_TEMP.int(2)\<^sub>s)\<close> \<open>x_2 \<le> snd (thm2_TEMP.int(2)\<^sub>s) \<longrightarrow> S x_1 x_2 \<le> S (snd (thm2_TEMP.int(1)\<^sub>s)) (snd (thm2_TEMP.int(2)\<^sub>s))\<close> by linarith
 qed
+
+(*If this holds, we are all good, in terms of the proof: *)
+(*lemma "\<And> x_1 :: real. x_1 \<ge> 5 \<Longrightarrow> False" 
+proof - 
+  fix x_1 :: real
+  have "x_1 \<ge> 5 \<longrightarrow> False" *)
+
+lemma "\<forall> x_1 :: real. x_1 \<ge> 5 \<Longrightarrow> False"
+  using not_numeral_le_neg_numeral by blast
+
 
 
 (*Rewrite this using our interval definitions, and f_ann, and spec_f. *)
@@ -149,30 +184,30 @@ theorem controller_conformance:
     "\<epsilon> \<ge> 0" and
 
     (*Assumptions on the normalisation, that the ranges are well-formed*)
-    "\<forall> i . snd(outRanges ! i) > fst(outRanges ! i) \<and> snd(annRange) > fst(annRange)" and
+    "\<forall> i :: nat. snd(outRanges ! i) > fst(outRanges ! i) \<and> 
+          snd(inRanges ! i) > fst(inRanges ! i) \<and> snd(annRange) > fst(annRange)" and
 
     (*The assumption on the range of the variables, we need them to be within the defined input ranges. *)
-    "\<And> x_1 x_2. x_1 \<ge> (inRanges(1).1) \<and>
-          x_1 \<le> (inRanges(1).2) \<and>
-          x_2 \<ge> (inRanges(2).1) \<and>
-          x_2 \<le> (inRanges(2).2)" and
   
     (*Marabou, these are the actual assumption discharged by Marabou: *)
-    "\<And> x_1 x_2. x_1 \<ge> normI 1 (inRanges(1).1) \<and> 
+    "\<And> x_1 x_2 :: real. x_1 \<ge> normI 1 (inRanges(1).1) \<and> 
           x_1 \<le> normI 1 (inRanges(1).2) \<and>
           x_2 \<ge> normI 2 (inRanges(2).1) \<and>
           x_2 \<le> normI 2 (inRanges(2).2) \<longrightarrow>
-          \<not> annout 2 1 [x_1, x_2] \<ge> normO 1 ((denormI 1 (normI 1 (inRanges(1).1) * P) + (denormI 2 (normI 2 (inRanges(2).1)) * D) ) + \<epsilon>)
+          \<not> annout 2 1 [x_1, x_2] \<ge> normO 1 ((P * denormI 1 (fst(int(1))) + (D * denormI 2 (fst(int(2)))) ) + \<epsilon>)
           " and
-    "\<And> x_1 x_2. x_1 \<ge> normI 1 (inRanges(1).1) \<and>
+    "\<And> x_1 x_2 :: real. x_1 \<ge> normI 1 (inRanges(1).1) \<and>
           x_1 \<le> normI 1 (inRanges(1).2) \<and>
           x_2 \<ge> normI 2 (inRanges(2).1) \<and>
           x_2 \<le> normI 2 (inRanges(2).2) \<longrightarrow>
-          \<not> annout 2 1 [x_1, x_2] \<le> normO 1 ((denormI 1 (normI 1 (inRanges(1).2) * P) + (denormI 2 (normI 2 (inRanges(2).2)) * D) ) - \<epsilon>)"
+          \<not> annout 2 1 [x_1, x_2] \<le> normO 1 ((P * denormI 1 (snd(int(1))) + (D * denormI 2 (snd(int(2)))) ) - \<epsilon>)"
     and 
-    "P > 0 \<and> D > 0"
-    
-shows "(conf_sin \<epsilon> angleOutputE AnglePIDANN AnglePID_C)" 
+    "P > 0 \<and> D > 0" 
+
+  shows "\<And> x_1 x_2 :: real. x_1 \<ge> normI 1 (inRanges(1).1) \<and> 
+          x_1 \<le> normI 1 (inRanges(1).2) \<and>
+          x_2 \<ge> normI 2 (inRanges(2).1) \<and>
+          x_2 \<le> normI 2 (inRanges(2).2) \<Longrightarrow> (conf_sin \<epsilon> angleOutputE AnglePIDANN AnglePID_C)" 
   apply (rule conf_vcs)
   (*Discharge first assumption: *)
    apply (simp add: assms(1))
@@ -180,39 +215,158 @@ shows "(conf_sin \<epsilon> angleOutputE AnglePIDANN AnglePID_C)"
 proof - 
   (*Start with some fixed variables, we have no assumptions about them here: *)
   fix x_1 x_2 y_1 :: real
-  from assms(4) assms(5) have m3: "x_1 \<ge> normI 1 (inRanges(1).1) \<and> 
+  assume 1: "x_1 \<ge> normI 1 (inRanges(1).1) \<and> 
+          x_1 \<le> normI 1 (inRanges(1).2) \<and>
+          x_2 \<ge> normI 2 (inRanges(2).1) \<and>
+          x_2 \<le> normI 2 (inRanges(2).2)"
+    (*This is the ultimate goal: *)
+  (*show "y_1 = P * x_1 + D * x_2 \<longrightarrow> \<bar>denormO 1 (annout 2 1 [normI 1 x_1, normI 2 x_2]) - y_1\<bar> \<le> \<epsilon>"
+     by sorry*)
+
+  from 1 have "denormO 1 x_1 \<ge> denormO 1 ( normI 1 (inRanges(1).1)) \<and> 
+          denormO 1 x_1 \<le> denormO 1 (normI 1 (inRanges(1).2)) \<and>
+          denormO 1 x_2 \<ge> denormO 1 (normI 2 (inRanges(2).1)) \<and>
+          denormO 1 x_2 \<le> denormO 1 (normI 2 (inRanges(2).2))" apply (simp add: mono_denormO)
+    by (metis assms(2) denormO_def diff_Suc_1 less_eq_real_def mono_norm)
+
+  from assms(3) assms(4) have m3: "x_1 \<ge> normI 1 (inRanges(1).1) \<and> 
           x_1 \<le> normI 1 (inRanges(1).2) \<and>
           x_2 \<ge> normI 2 (inRanges(2).1) \<and>
           x_2 \<le> normI 2 (inRanges(2).2) \<longrightarrow>
       
-          \<not> annout 2 1 [x_1, x_2] \<ge> normO 1 ((denormI 1 (normI 1 (inRanges(1).1) * P) + (denormI 2 (normI 2 (inRanges(2).1)) * D) ) + \<epsilon>)
+          \<not> annout 2 1 [x_1, x_2] \<ge> normO 1 ((P * denormI 1 (fst(int(1))) + (D * denormI 2 (fst(int(2)))) ) + \<epsilon>)
            \<and>
-          \<not> annout 2 1 [x_1, x_2] \<le> normO 1 ((denormI 1 (normI 1 (inRanges(1).2) * P) + (denormI 2 (normI 2 (inRanges(2).2)) * D) ) - \<epsilon>)"
+          \<not> annout 2 1 [x_1, x_2] \<le> normO 1 ((P * denormI 1 (snd(int(1))) + (D * denormI 2 (snd(int(2)))) ) - \<epsilon>)"
     by auto
     
    have "... \<longrightarrow>
-   (annout 2 1 [x_1, x_2] \<le> (normO 1 ((denormI 1 (normI 1 (inRanges(1).1) * P) + (denormI 2 (normI 2 (inRanges(2).1)) * D) ))) + \<epsilon>)
+   annout 2 1 [x_1, x_2] \<le> normO 1 ((P * denormI 1 (fst(int(1))) + (D * denormI 2 (fst(int(2)))) ) + \<epsilon>)
      \<and>
-    (annout 2 1 [x_1, x_2] \<ge> (normO 1 ((denormI 1 (normI 1 (inRanges(1).2) * P) + (denormI 2 (normI 2 (inRanges(2).2)) * D) ))) - \<epsilon>)"
-     by (smt (z3) assms(3))
-
-  (*Very important step now, *)
+    annout 2 1 [x_1, x_2] \<ge> normO 1 ((P * denormI 1 (snd(int(1))) + (D * denormI 2 (snd(int(2)))) ) - \<epsilon>)"
+     using nle_le by blast
+     
 
    have "... \<longrightarrow> 
-      (annout 2 1 [x_1, x_2] \<ge> (normO 1 ((denormI 1 (x_1 * P) + (denormI 2 (x_2 * D) ))) - \<epsilon>))
+     annout 2 1 [x_1, x_2] \<le> normO 1 (norm_spec_f_2 (fst(int(1))) (fst(int(2))) + \<epsilon>)
      \<and> 
-     (annout 2 1 [x_1, x_2] \<le> (normO 1 ((denormI 1 (x_1 * P) + (denormI 2 (x_2 * D) ))) + \<epsilon>))
+     annout 2 1 [x_1, x_2] \<ge> normO 1 (norm_spec_f_2 (snd(int(1))) (snd(int(2))) - \<epsilon>)
+    "
+     unfolding norm_spec_f_2_def
+     apply (simp)
+     done
+
+   have "... \<longrightarrow> 
+     annout 2 1 [x_1, x_2] \<ge> normO 1 (norm_spec_f_2 (snd(int(1))) (snd(int(2))) - \<epsilon>)
+      \<and> 
+     annout 2 1 [x_1, x_2] \<le> normO 1 (norm_spec_f_2 (fst(int(1))) (fst(int(2))) + \<epsilon>)
+     
+    "
+     apply (simp)
+     done
+  
+  (*Important step, get from the intervals to the actual fixed variables: *)
+   have "... \<longrightarrow> 
+     annout 2 1 [x_1, x_2] \<ge> normO 1 (norm_spec_f_2 (x_1) (x_2) - \<epsilon>)
+     \<and> 
+     annout 2 1 [x_1, x_2] \<le> normO 1 (norm_spec_f_2 (x_1) (x_2) + \<epsilon>)
     "
      apply (rule impI)
      apply (rule spec_mono_ann)
-     sorry
+   proof - 
+     show "\<forall> x_1 x_2 y_1 y_2. x_1 \<le> y_1 \<and> x_2 \<le> y_2 \<longrightarrow> norm_spec_f_2 x_1 x_2 \<le> norm_spec_f_2 y_1 y_2" 
+       using assms apply (simp add: norm_spec_f_2_mono)
+       done
+
+     show "fst (int(1)) \<le> x_1 \<and> x_1 \<le> snd (int(1))" 
+       using 1 by (simp add: int_def)
+
+     show "fst (int(2)\<^sub>s) \<le> x_2  \<and> x_2 \<le> snd (int(2)\<^sub>s)" 
+        using 1 by (simp add: int_def)
+
+    show "0 \<le> \<epsilon>" 
+       using assms by simp
+
+     show "0 < P \<and> 0 < D" 
+          using assms by simp
+     show "fst (outRanges ! 0) < snd (outRanges ! 0) \<and> fst annRange < snd annRange" using assms by simp
+
+
+     assume "annout 2 1 [x_1, x_2] \<ge> normO 1 (norm_spec_f_2 (snd(int(1))) (snd(int(2))) - \<epsilon>)
+      \<and> 
+     annout 2 1 [x_1, x_2] \<le> normO 1 (norm_spec_f_2 (fst(int(1))) (fst(int(2))) + \<epsilon>)"
+     show 
+     "f_ann x_1 x_2 \<le> normO 1 (norm_spec_f_2 (fst (int(1))) (fst (int(2))) + \<epsilon>) \<and>
+      f_ann x_1 x_2 \<ge> normO 1 (norm_spec_f_2 (snd (int(1))) (snd (thm2_TEMP.int(2))) - \<epsilon>)"
+       using \<open>normO 1 (norm_spec_f_2 (snd (thm2_TEMP.int(1)\<^sub>s)) (snd (thm2_TEMP.int(2)\<^sub>s)) - \<epsilon>) \<le> f_ann x_1 x_2 \<and> f_ann x_1 x_2 \<le> normO 1 (norm_spec_f_2 (fst (thm2_TEMP.int(1)\<^sub>s)) (fst (thm2_TEMP.int(2)\<^sub>s)) + \<epsilon>)\<close> by fastforce 
+   qed
+
+    
+    
+
+
+(*
+Premises we have to show: 
+          "fst(int(1)) \<le> x_1 \<and> x_1 \<le> snd(int(1))" and 
+          "fst(int(2)) \<le> x_2 \<and> x_2 \<le> snd(int(2))" and 
+          "(snd(outRanges ! 0) > fst(outRanges ! 0) \<and> snd(annRange) > fst(annRange))" and
+          "\<epsilon> > 0" and 
+          "P > 0 \<and> D > 0" and
+          "f_ann x_1 x_2 \<le> normO 1 (S (fst(int(1))) (fst(int(2))) + \<epsilon>)
+               \<and> f_ann x_1 x_2 \<ge> normO 1 (S (snd(int(1))) (snd(int(2))) - \<epsilon>) 
+              " and 
+          (*Monotonicity property for our specification function: *)
+          "\<forall> x_1 x_2 y_1 y_2 :: real. x_1 \<le> y_1 \<and> x_2 \<le> y_2 \<longrightarrow> S x_1 x_2 \<le> S y_1 y_2"
+*)
+     
+      
+      
+    have "... \<longrightarrow> 
+     (annout 2 1 [x_1, x_2] \<le> normO 1 (norm_spec_f_2 (x_1) (x_2) + \<epsilon>)
+     \<and> 
+     annout 2 1 [x_1, x_2] \<ge> normO 1 (norm_spec_f_2 (x_1) (x_2) - \<epsilon>))  
+    \<and> 
+    (
+          x_1 \<ge> normI 1 (inRanges(1).1) \<and> 
+          x_1 \<le> normI 1 (inRanges(1).2) \<and>
+          x_2 \<ge> normI 2 (inRanges(2).1) \<and>
+          x_2 \<le> normI 2 (inRanges(2).2)
+    )
+    "
+      using "1" by fastforce 
+
+  have "... \<longrightarrow> 
+     (annout 2 1 [x_1, x_2] \<le> normO 1 (norm_spec_f_2 (x_1) (x_2) + \<epsilon>)
+     \<and> 
+     annout 2 1 [x_1, x_2] \<ge> normO 1 (norm_spec_f_2 (x_1) (x_2) - \<epsilon>))  
+    \<and> 
+    (
+          denormI 1 x_1 \<ge> denormI 1 (normI 1 (inRanges(1).1)) \<and> 
+          denormI 1 x_1 \<le> denormI 1 (normI 1 (inRanges(1).2)) \<and>
+          denormI 2 x_2 \<ge> denormI 2 (normI 2 (inRanges(2).1)) \<and>
+          denormI 2 x_2 \<le> denormI 2 (normI 2 (inRanges(2).2))
+    )
+    "
+    by (metis assms(2) less_eq_real_def mono_denormI)
+
+    have "... =
+     (annout 2 1 [x_1, x_2] \<le> normO 1 (norm_spec_f_2 (x_1) (x_2) + \<epsilon>)
+     \<and> 
+     annout 2 1 [x_1, x_2] \<ge> normO 1 (norm_spec_f_2 (x_1) (x_2) - \<epsilon>))  
+    \<and> 
+    (
+          denormI 1 x_1 \<ge> (inRanges(1).1) \<and> 
+          denormI 1 x_1 \<le> (inRanges(1).2) \<and>
+          denormI 1 x_2 \<ge> (inRanges(2).1) \<and>
+          denormI 1 x_2 \<le> (inRanges(2).2)
+    )
+    " input_norm2
+      
 
 
 
    (********************************)
 
-  (*This is the ultimate goal: *)
-  show "y_1 = P * x_1 + D * x_2 \<longrightarrow> \<bar>denormO 1 (annout 2 1 [normI 1 x_1, normI 2 x_2]) - y_1\<bar> \<le> \<epsilon>" by sorry
+
 qed
 
 
